rustexamples/test/49_mut_ref_invariant_imprecise.rs
@@ -1,0 +1,21 @@
+//rustc +nightly 49_mut_ref_invariant_imprecise.rs -Z polonius=next
+
+// A variant of 36.rs where we use mutable reference to illustrate the
+// imprecision of invariant for mutable reference. Both Polonius and
+// our borrow checker reject this program. 
+
+fn main(){
+    let mut v1: i32 = 1;
+    let mut v2: i32 = 2;
+    let mut p1: &mut i32 = &mut v1;
+    let mut p2: &mut i32 = &mut v2;
+    let mut q : &mut & mut i32;
+    if true {
+        q = &mut p1;
+    } else {
+        q = &mut p2;
+    }
+    let mut tmp: i32 = **q;
+    v1 = 2; 
+    tmp = *p2; // If we uncomment this line, there would be error at the last line
+}
